\documentclass{ximera}

\input{../../preamble.tex}
\author{Bobby Ramsey}

\begin{document}
\begin{exercise}
	Find the derivative of $\displaystyle f(x) = 4e^{2x+1}-6x$.
	
	\[ f'(x) = \answer{8e^{2x+1}-6} \]
\end{exercise}

\begin{exercise}
	Find the derivative of $\displaystyle g(y) = (6y^2-1)e^{\sqrt{y}}$.

	\[ g'(y) = \answer{(12y)e^{\sqrt{y}} +\frac{6y^2-1}{2\sqrt{y}}e^{\sqrt{y}}  }\]
\end{exercise}

\begin{exercise}
	Find the derivative of $\displaystyle h(t) = \dfrac{2te^{-t}}{t^2+1}$.
	
	\[ h'(t) = \answer{ \frac{(2e^{-t}-2te^{-t})(t^2+1)-(2t)(2te^{-t})}{(t^2+1)^2}} \]
\end{exercise}



\end{document}

