\documentclass{ximera}
\input{../../preamble.tex}
\author{Emma Smith Zbarsky}
\license{Creative Commons Attribution 3.0 Unported}
\acknowledgement{https://quadbase.org/questions/q14513v1}
\begin{document}

\begin{exercise}

Find $y(t)$ if $y'(t) = 3t^7-4t^3$ and $y(0)=-6$.


\begin{hint}
This is an initial value problem. First, find the general antiderivative
and then use the given initial condition to solve for the particular
antiderivative that satisfies the initial condition.
\end{hint}


\begin{hint}
\begin{align*}
\int y'(t)\; dt &= \int 3t^7-4t^3\; dt \\
y(t) &= \frac{3}{8}t^8-t^4+C \\
y(0) = -6 &= \frac{3}{8}(0^8)-0^4+C \\
& \Rightarrow C=-6 \\
y(t) &= \frac{3}{8}t^8-t^4-6 
\end{align*}
\end{hint}


\begin{multipleChoice}
\choice{$y(t) = 21t^6-12t^2-6$}
\choice[correct]{$y(t) = \frac{3}{8}t^8-t^4-6$}
\choice{$y(t) = \frac{3}{8}t^8-t^4$}
\choice{$y(t) = \frac{3}{8}t^8-t^4+C$}
\choice{$y(t) = 21t^6-12t^2$}
\end{multipleChoice}

\end{exercise}
\end{document}
