\documentclass{ximera}

\input{../../preamble.tex}

\author{Carl Stitz \and Jeff Zeager \and Bart Snapp \and Matthew Carr}
\license{CC-By-SA-NC}
\acknowledgement{http://www.stitz-zeager.com/}

\begin{document}
\begin{exercise}

\outcome{Work with exponential and logarithmic functions.}
\outcome{Know and use the properties of exponential and logarithmic functions.}

\tag{logarithms}




Use the properties of logarithms to write the expression as a single
logarithm. 

\begin{enumerate}
	\item $4\ln(x) + 2\ln(y)=\answer{\ln(x^4y^2)}$ 
	
	\item $\log_{2}(x) + \log_{2}(y) - \log_{2}(z)=\answer{\log_{2}(\frac{xy}{z})}$
	
	\item $\log_{3}(x) - 2 \log_{3}(y)=\answer{\log_{3}(\frac{x}{y^2})}$
	
	\item $\frac{1}{2}\log_{3}(x) - 2\log_{3}(y) - \log_{3}(z)=\answer{\log_{3}(\frac{\sqrt{x}}{y^2 z})}$
	
	\item $2 \ln(x) -3 \ln(y) - 4\ln(z)=\answer{\ln(\frac{x^2}{y^3z^4})}$
	
	\item $\ln(x) - \frac{1}{4} \ln(z) + \frac{1}{2} \ln(y)=\answer{\ln(\frac{x\sqrt{y}}{\sqrt[4]{z}})}$
	
	\item $-\frac{1}{2} \ln(x) - \frac{1}{2}\ln(y) - \frac{1}{2} \ln(z)=\answer{\ln(\frac{1}{\sqrt{xyz}})}$
	
	\item $\log_{5}(x) - 3=\answer{\log_{5}(\frac{x}{125})}$
	
	\item $\log_{7}(x) + \log_{7}(x - 3) - 2=\answer{\log_{7}(\frac{x(x-3)}{49})}$
	
	\item $\ln(x) + \frac{1}{2}=\answer{\ln(x\sqrt{e})}$ 
	
	\item $\log_{2}(x) + \log_{4}(x)=\answer{\log_{4}(x^{3})}$ 
	
	\item $\log_{2}(x) + \log_{4}(x-1)=\answer{\log_{4}(x^2(x-1))}$
	
	\item $\log_{2}(x) + \log_{\frac{1}{2}}(x - 1)=\answer{\log_{2}(\frac{x}{x-1})}$ 
\end{enumerate}

\end{exercise}
\end{document}

