\documentclass{ximera}

\input{../../preamble.tex}
\author{Bobby Ramsey}

\begin{document}
\begin{exercise}
	Solve the equation.
	\[ 2e^{2x} + e^x  = 9 - 2 e^x \]
	There is/are $\answer{1}$ solution(s).
	\begin{hint}
		Start by moving everything to the left-hand side.  
		\[ 2e^{2x}+3e^x-9 = 0 \]
		Notice that $e^{2x}$ is really just $(e^x)^2$?  Make a substitution $u = e^x$.
	\end{hint}
	\begin{exercise}
		Enter your solution.
		Solutions: $x = \answer{ \ln(3/2) }$.
	\end{exercise}
\end{exercise}

\end{document}

